theories/examples/while.v
@@ -2,11 +2,14 @@ From gitrees Require Import prelude gitree.
 
 Section while.
   Context {E : opsInterp}.
-  Notation IT := (IT E natO).
-  Notation ITV := (ITV E natO).
+  Context {R} `{!Cofe R}.
+  Context `{!SubOfe unitO R}.
+  Context `{!SubOfe natO R}.
+  Notation IT := (IT E R).
+  Notation ITV := (ITV E R).
 
   Program Definition pre_while (while : IT -n> IT -n> IT) : IT -n> IT -n> IT :=
-    λne cond body, IF cond (SEQ body (Tick (while cond body))) (Nat 0).
+    λne cond body, IF cond (SEQ body (Tick (while cond body))) (Ret ()).
   Solve All Obligations with solve_proper_please.
 
   #[local] Instance pre_while_contractive : Contractive pre_while.
@@ -15,7 +18,11 @@ Section while.
 
   (** WHILE (α > 0) DO β *)
   Lemma WHILE_eq α β :
-    WHILE α β ≡ IF α (SEQ β (Tick (WHILE α β))) (Nat 0).
-  Proof. apply (fixpoint_unfold pre_while _ _). Qed.
+    WHILE α β ≡ IF α (SEQ β (Tick (WHILE α β))) (Ret ()).
+  Proof.
+    etrans.
+    - apply (fixpoint_unfold pre_while _ _).
+    - reflexivity.
+  Qed.
 
 End while.
