theories/gitree/lambda.v
@@ -3,19 +3,146 @@ From iris.prelude Require Import options.
 From iris.base_logic Require Export base_logic.
 From gitrees Require Import prelude gitree.core.
 
+Class SubOfe (A B : ofe) := { subOfe_rest : ofe; subOfe_in : ofe_iso (sumO A subOfe_rest) B }.
+
+Program Definition Empty_setO_rec A : Empty_setO -n> A := λne x, Empty_set_rect (λ _, A) x.
+Next Obligation. intros A n x y. inversion x. Qed.
+
+Definition sumO_assoc A B C : sumO A (sumO B C) ≃ sumO (sumO A B) C.
+Proof.
+  simple refine (OfeIso _ _ _ _).
+  - refine (sumO_rec (inlO ◎ inlO) _).
+    refine (sumO_rec (inlO ◎ inrO) inrO).
+  - refine (sumO_rec _ (inrO ◎ inrO)).
+    refine (sumO_rec inlO (inrO ◎ inlO)).
+  - intros [[?|?]|?]; simpl; eauto.
+  - intros [?|[?|?]]; simpl; eauto.
+Defined.
+Definition sumO_compat_l A B C : A ≃ B → sumO A C ≃ sumO B C.
+Proof.
+  intros f.
+  simple refine (OfeIso _ _ _ _).
+  - refine (sumO_rec (inlO ◎ f) inrO).
+  - refine (sumO_rec (inlO ◎ f^-1) inrO).
+  - intros [?|?]; simpl; eauto.
+    rewrite ofe_iso_12//.
+  - intros [?|?]; simpl; eauto.
+    rewrite ofe_iso_21//.
+Defined.
+Definition sumO_sym A B : sumO A B ≃ sumO B A.
+Proof.
+  simple refine (OfeIso _ _ _ _).
+  - refine (sumO_rec inrO inlO).
+  - refine (sumO_rec inrO inlO).
+  - intros [?|?]; simpl; eauto.
+  - intros [?|?]; simpl; eauto.
+Defined.
+Definition sumO_unitO_r A : sumO A Empty_setO ≃ A.
+Proof.
+  simple refine (OfeIso _ inlO _ _).
+  - refine (sumO_rec cid (Empty_setO_rec _)).
+  - simpl. eauto.
+  - intros [?|?]; simpl; eauto. inversion o.
+Defined.
+
+#[global] Instance subOfe_id A : SubOfe A A.
+Proof.
+  refine ({| subOfe_rest := Empty_setO |}).
+  apply sumO_unitO_r.
+Defined.
+
+#[global] Instance subOfe_inl A B C `{!SubOfe A B} : SubOfe A (sumO B C).
+Proof.
+  refine ({| subOfe_rest := sumO subOfe_rest C |}).
+  eapply iso_ofe_trans.
+  { apply sumO_assoc. }
+  apply sumO_compat_l. apply subOfe_in.
+Defined.
+#[global] Instance subOfe_inr A B C `{!SubOfe A B} : SubOfe A (sumO C B).
+Proof.
+  refine ({| subOfe_rest := sumO subOfe_rest C |}).
+  eapply iso_ofe_trans.
+  { apply sumO_assoc. }
+  eapply iso_ofe_trans.
+  { apply sumO_compat_l. apply subOfe_in. }
+  apply sumO_sym.
+Defined.
+#[global] Hint Mode SubOfe ! ! : typeclass_instances.
+
+Section it_subofe.
+  Context {E : opsInterp}.
+  Context {A B : ofe} `{!Cofe A, !Cofe B} `{!SubOfe A B}.
+  Notation IT := (IT E B).
+
+  Definition Ret : A -n> IT := Ret ◎ subOfe_in ◎ inlO.
+  Program Definition RetV : A -n> ITV E B := OfeMor RetV ◎ subOfe_in ◎ inlO.
+  Definition get_ret (f : A -n> IT) : IT -n> IT := get_ret (sumO_rec f Err1 ◎ subOfe_in^-1).
+
+  #[global] Instance get_ret_ne n : Proper ((dist n) ==> (dist n)) get_ret.
+  Proof.
+    repeat intro. unfold get_ret. solve_proper.
+  Qed.
+  #[global] Instance get_ret_proper : Proper ((≡) ==> (≡)) get_ret.
+  Proof.
+    repeat intro. unfold get_ret. solve_proper.
+  Qed.
+
+  Program Definition get_ret2 (f : A -n> A -n> IT) : IT -n> IT -n> IT := λne x y,
+      get_ret (λne x, get_ret (λne y, f x y) y) x.
+  Solve All Obligations with solve_proper_please.
+  Global Instance get_ret2_ne n : Proper ((dist n) ==> (dist n)) get_ret2.
+  Proof.
+    intros f1 f2 Hf. unfold get_ret2.
+    intros x y. simpl. apply get_ret_ne.
+    clear x. intros x. simpl. apply get_ret_ne.
+    clear y. intros y. simpl. apply Hf.
+  Qed.
+  Global Instance get_ret2_proper : Proper ((≡) ==> (≡)) get_ret2.
+  Proof.
+    intros f1 f2 Hf. unfold get_ret2.
+    intros x y. simpl. apply get_ret_proper.
+    clear x. intros x. simpl. apply get_ret_proper.
+    clear y. intros y. simpl. apply Hf.
+  Qed.
+
+  Lemma get_ret_ret f n : get_ret f (Ret n) ≡ f n.
+  Proof.
+    rewrite get_ret_ret. cbn-[sumO_rec].
+    rewrite ofe_iso_21. done.
+  Qed.
+
+  Lemma get_val_ret f n : get_val f (Ret n) ≡ f (Ret n).
+  Proof. by rewrite IT_rec1_ret. Qed.
+  Lemma get_fun_ret f n : get_fun f (Ret n) ≡ Err RuntimeErr.
+  Proof. by rewrite IT_rec1_ret. Qed.
+
+  Lemma IT_of_V_Ret n : IT_of_V (RetV n) ≡ Ret n.
+  Proof. done. Qed.
+  Lemma IT_to_V_Ret n : IT_to_V (Ret n) ≡ Some (RetV n).
+  Proof. simpl. rewrite IT_to_V_Ret. done. Qed.
+
+  #[export] Instance intoval_ret n : IntoVal (Ret n) (RetV n).
+  Proof. unfold IntoVal. simpl. reflexivity. Qed.
+  #[export] Instance asval_ret n : AsVal (Ret n).
+  Proof. exists (RetV n). reflexivity. Qed.
+
+  #[global] Opaque Ret RetV.
+End it_subofe.
+
 Section lambda.
   Local Opaque laterO_ap.
 
-  Context {Σ : opsInterp}.
+  Context {Σ : opsInterp} {A : ofe} `{!Cofe A}.
 
-  Notation IT := (IT Σ natO).
+  Notation IT := (IT Σ A).
 
-  Program Definition IF : IT -n> IT -n> IT -n> IT := λne t t1 t2,
-      get_nat (λ n, if Nat.ltb 0 n then t1 else t2) t.
-  Solve All Obligations with solve_proper.
+  Program Definition IF `{!SubOfe natO A} : IT -n> IT -n> IT -n> IT := λne t t1 t2,
+      get_ret (λne n, if Nat.ltb 0 n then t1 else t2) t.
+  Next Obligation. repeat intro. by rewrite H. Qed.
+  Solve All Obligations with solve_proper_please.
 
-  Program Definition IF_last : IT -n> IT -n> IT -n> IT := λne t1 t2 t, IF t t1 t2.
-  Solve All Obligations with solve_proper.
+  Program Definition IF_last `{!SubOfe natO A} : IT -n> IT -n> IT -n> IT := λne t1 t2 t, IF t t1 t2.
+  Solve All Obligations with solve_proper_please.
 
   (** A non-strict application, does not recurse under the effects of the argument *)
   Program Definition APP : IT -n> laterO IT -n> IT := λne f x,
@@ -32,10 +159,10 @@ Section lambda.
   (** We define the interpretation of NatOp in two stages.
       First, we recurse under ticks and visitors in both arguments, and only then perform the op
    *)
-  Program Definition NATOP (f : nat → nat → nat) : IT -n> IT -n> IT := λne t1 t2,
+  Program Definition NATOP `{!SubOfe natO A} (f : nat → nat → nat) : IT -n> IT -n> IT := λne t1 t2,
       get_val (λne v2,
         get_val (λne v1,
-                   get_nat2 (λ n1 n2, Nat (f n1 n2)) v1 v2) t1) t2.
+                   get_ret2 (λne n1 n2, Ret (f n1 n2)) v1 v2) t1) t2.
   Solve All Obligations with solve_proper_please.
 
   (** Sequencing *)
@@ -46,8 +173,8 @@ Section lambda.
   Program Definition LET : IT -n> (IT -n> IT) -n> IT := λne x f, get_val f x.
   Solve Obligations with solve_proper.
 
-  Lemma APP_Nat x y : APP (Ret x) y ≡ Err RuntimeErr.
-  Proof. simpl. by rewrite get_fun_ret. Qed.
+  Lemma APP_Ret x y : APP (core.Ret x) y ≡ Err RuntimeErr.
+  Proof. simpl. by rewrite core.get_fun_ret. Qed.
   Lemma APP_Err e x : APP (Err e) x ≡ Err e.
   Proof. simpl. by rewrite get_fun_err. Qed.
   Lemma APP_Fun f x : APP (Fun f) x ≡ Tau $ laterO_ap f x.
@@ -69,8 +196,8 @@ Section lambda.
   Qed.
   Lemma APP'_Err_r f e : APP' f (Err e) ≡ Err e.
   Proof. simpl. by rewrite get_val_err. Qed.
-  Lemma APP'_Nat_r f x : APP' f (Ret x) ≡ APP f (Next (Ret x)).
-  Proof. simpl. rewrite get_val_ret. done. Qed.
+  Lemma APP'_Ret_r f x : APP' f (core.Ret x) ≡ APP f (Next (core.Ret x)).
+  Proof. simpl. rewrite core.get_val_ret. done. Qed.
   Lemma APP'_Fun_r f x : APP' f (Fun x) ≡ APP f (Next (Fun x)).
   Proof. simpl. rewrite get_val_fun. done. Qed.
   Lemma APP'_Tick_r f t : APP' f (Tick t) ≡ Tick $ APP' f t.
@@ -81,11 +208,11 @@ Section lambda.
   Qed.
   Lemma APP'_Vis_r f op i k : APP' f (Vis op i k) ≡ Vis op i (laterO_map (APP' f) ◎ k).
   Proof. by rewrite get_val_vis. Qed.
-  Lemma APP_APP'_ITV' α (βv : ITV Σ natO) :
+  Lemma APP_APP'_ITV' α (βv : ITV Σ A) :
     APP' α (IT_of_V βv) ≡ APP α (Next (IT_of_V βv)).
   Proof.
     destruct βv as [n|f]; simpl.
-    - rewrite APP'_Nat_r//.
+    - rewrite APP'_Ret_r//.
     - rewrite APP'_Fun_r//.
   Qed.
   (* XXX: the names here are weird *)
@@ -110,38 +237,36 @@ Section lambda.
   Qed.
   Lemma APP'_Err_l e x `{!AsVal x}: APP' (Err e) x ≡ Err e.
   Proof. rewrite APP_APP'_ITV. by rewrite APP_Err. Qed.
-  Lemma APP'_Nat_l x t `{!AsVal t}: APP' (Ret x) t ≡ Err RuntimeErr.
-  Proof. rewrite APP_APP'_ITV. by rewrite APP_Nat. Qed.
+  Lemma APP'_Ret_l x t `{!AsVal t}: APP' (core.Ret x) t ≡ Err RuntimeErr.
+  Proof. rewrite APP_APP'_ITV. by rewrite APP_Ret. Qed.
   Lemma APP'_Fun_l f x `{!AsVal x} : APP' (Fun f) x ≡ Tau $ laterO_ap f (Next x).
   Proof. rewrite APP_APP'_ITV. by rewrite APP_Fun. Qed.
 
-  Lemma IF_Err e t1 t2 : IF (Err e) t1 t2 ≡ Err e.
+  Lemma IF_Err `{!SubOfe natO A} e t1 t2 : IF (Err e) t1 t2 ≡ Err e.
   Proof. unfold IF. simpl. by rewrite get_ret_err. Qed.
-  Lemma IF_True n t1 t2 :
+  Lemma IF_True `{!SubOfe natO A} n t1 t2 :
     0 < n → IF (Ret n) t1 t2 ≡ t1.
   Proof.
     intro Hn. unfold IF. simpl.
-    rewrite get_ret_ret. simpl.
-    assert (0 <? n = true) as ->; last by eauto.
-    by apply Nat.ltb_lt.
+    rewrite get_ret_ret.
+    destruct n; first lia; last eauto.
   Qed.
-  Lemma IF_False n t1 t2 :
+  Lemma IF_False `{!SubOfe natO A} n t1 t2 :
     0 ≥ n → IF (Ret n) t1 t2 ≡ t2.
   Proof.
     intro Hn. unfold IF. simpl.
-    rewrite get_ret_ret. simpl.
-    assert (0 <? n = false) as ->; last by eauto.
-    by apply Nat.ltb_ge.
+    rewrite get_ret_ret.
+    destruct n; first eauto; last lia.
   Qed.
-  Lemma IF_Tick t t1 t2 :
+  Lemma IF_Tick `{!SubOfe natO A} t t1 t2 :
     IF (Tick t) t1 t2 ≡ Tick (IF t t1 t2).
   Proof. rewrite {1}/IF /=. apply get_ret_tick. Qed.
-  Lemma IF_Tick_n n t t1 t2 :
+  Lemma IF_Tick_n `{!SubOfe natO A} n t t1 t2 :
     IF (Tick_n n t) t1 t2 ≡ Tick_n n (IF t t1 t2).
   Proof.
     induction n; eauto. by rewrite IF_Tick IHn.
   Qed.
-  Lemma IF_Vis op i k t1 t2 :
+  Lemma IF_Vis `{!SubOfe natO A} op i k t1 t2 :
     IF (Vis op i k) t1 t2 ≡ Vis op i (laterO_map (IF_last t1 t2) ◎ k).
   Proof.
     rewrite {1}/IF /=.
@@ -149,14 +274,14 @@ Section lambda.
     by intro.
   Qed.
 
-  Lemma NATOP_Err_r f e t1 : NATOP f t1 (Err e) ≡ Err e.
+  Lemma NATOP_Err_r `{!SubOfe natO A} f e t1 : NATOP f t1 (Err e) ≡ Err e.
   Proof. simpl. by rewrite get_val_err. Qed.
-  Lemma NATOP_Err_l f e β : AsVal β → NATOP f (Err e) β ≡ Err e.
+  Lemma NATOP_Err_l `{!SubOfe natO A} f e β : AsVal β → NATOP f (Err e) β ≡ Err e.
   Proof.
     intros ?. simpl.
     rewrite get_val_ITV /= get_val_err //.
   Qed.
-  Lemma NATOP_Ret n1 n2 f :
+  Lemma NATOP_Ret `{!SubOfe natO A} n1 n2 f :
     NATOP f (Ret n1) (Ret n2) ≡ Ret (f n1 n2).
   Proof.
     simpl.
@@ -165,18 +290,18 @@ Section lambda.
     rewrite !get_ret_ret. simpl.
     done.
   Qed.
-  Lemma NATOP_Tick_r t1 t2 f :
+  Lemma NATOP_Tick_r `{!SubOfe natO A} t1 t2 f :
     NATOP f t1 (Tick t2) ≡ Tick $ NATOP f t1 t2.
   Proof.
     simpl. rewrite get_val_tick//.
   Qed.
-  Lemma NATOP_Tick_n_r t1 t2 f n :
+  Lemma NATOP_Tick_n_r `{!SubOfe natO A} t1 t2 f n :
     NATOP f t1 (Tick_n n t2) ≡ Tick_n n $ NATOP f t1 t2.
   Proof.
     induction n; eauto. rewrite NATOP_Tick_r.
     rewrite IHn. done.
   Qed.
-  Lemma NATOP_ITV_Tick_l t1 β f :
+  Lemma NATOP_ITV_Tick_l `{!SubOfe natO A} t1 β f :
     AsVal β →
     NATOP f (Tick t1) β ≡ Tick $ NATOP f t1 β.
   Proof.
@@ -184,7 +309,7 @@ Section lambda.
     rewrite get_val_tick. f_equiv.
     rewrite get_val_ITV. done.
   Qed.
-  Lemma NATOP_ITV_Tick_n_l t1 β f n :
+  Lemma NATOP_ITV_Tick_n_l `{!SubOfe natO A} t1 β f n :
     AsVal β →
     NATOP f (Tick_n n t1) β ≡ Tick_n n $ NATOP f t1 β.
   Proof.
@@ -192,12 +317,12 @@ Section lambda.
     induction n; eauto. rewrite NATOP_ITV_Tick_l.
     rewrite IHn. done.
   Qed.
-  Lemma NATOP_Vis_r t1 op i k f :
+  Lemma NATOP_Vis_r `{!SubOfe natO A} t1 op i k f :
     NATOP f t1 (Vis op i k) ≡ Vis op i (laterO_map (NATOP f t1) ◎ k).
   Proof.
     simpl. rewrite get_val_vis. f_equiv. solve_proper.
   Qed.
-  Lemma NATOP_ITV_Vis_l op i k β f :
+  Lemma NATOP_ITV_Vis_l `{!SubOfe natO A} op i k β f :
     AsVal β →
     NATOP f (Vis op i k) β ≡
     Vis op i (laterO_map (flipO (NATOP f) β) ◎ k).
@@ -212,21 +337,21 @@ Section lambda.
   Lemma LET_Val α f `{!AsVal α} : LET α f ≡ f α.
   Proof. unfold LET. simpl. rewrite get_val_ITV//. Qed.
 
-  Global Instance IF_Proper : Proper ((≡) ==> (≡)) IF.
+  Global Instance IF_Proper `{!SubOfe natO A} : Proper ((≡) ==> (≡)) IF.
   Proof. apply ne_proper. apply _. Qed.
   Global Instance APP_Proper : Proper ((≡) ==> (≡)) APP.
   Proof. apply ne_proper. apply _. Qed.
   Global Instance APP'_Proper : Proper ((≡) ==> (≡)) APP'.
   Proof. apply ne_proper. apply _. Qed.
-  Global Instance NATOP_Proper f : Proper ((≡) ==> (≡)) (NATOP f).
+  Global Instance NATOP_Proper `{!SubOfe natO A} f : Proper ((≡) ==> (≡)) (NATOP f).
   Proof. apply ne_proper. apply _. Qed.
 
   Opaque APP APP' IF NATOP.
   Definition AppLSCtx (β α : IT) := APP' α β.
   Definition AppRSCtx (β α : IT) := APP' β α.
-  Definition NatOpLSCtx f (β α : IT) := NATOP f α β.
-  Definition NatOpRSCtx f (β α : IT) := NATOP f β α.
-  Definition IFSCtx (β1 β2 α : IT) := IF α β1 β2.
+  Definition NatOpLSCtx `{!SubOfe natO A} f (β α : IT) := NATOP f α β.
+  Definition NatOpRSCtx `{!SubOfe natO A} f (β α : IT) := NATOP f β α.
+  Definition IFSCtx `{!SubOfe natO A} (β1 β2 α : IT) := IF α β1 β2.
   Definition SEQCtx (β2 α : IT) := SEQ α β2.
   Definition LETCTX f : IT -n> IT := λne x, LET x f.
 
@@ -251,27 +376,27 @@ Section lambda.
       by intro.
     - intros e. by rewrite APP'_Err_r.
   Qed.
-  #[local] Instance NatOpLSCtx_ne op (β : IT) : NonExpansive (NatOpLSCtx op β).
+  #[local] Instance NatOpLSCtx_ne op (β : IT) `{!SubOfe natO A} : NonExpansive (NatOpLSCtx op β).
   Proof.
     intro n. unfold NatOpLSCtx.
     repeat intro. repeat f_equiv; eauto.
   Qed.
-  #[export] Instance NatOpLSCtx_hom op (β : IT) : AsVal β → IT_hom (NatOpLSCtx op β).
+  #[export] Instance NatOpLSCtx_hom op (β : IT) `{!SubOfe natO A} `{!AsVal β} : IT_hom (NatOpLSCtx op β).
   Proof.
-    intros Hb. unfold NatOpLSCtx.
+    unfold NatOpLSCtx.
     simple refine (IT_HOM _ _ _ _ _).
     - intro a. simpl. rewrite NATOP_ITV_Tick_l//.
     - intros op' i k. simpl. rewrite NATOP_ITV_Vis_l//.
       repeat f_equiv. intro. reflexivity.
     - intros e. simpl. rewrite NATOP_Err_l//.
   Qed.
-  #[local] Instance NatOpRSCtx_ne op (β : IT) : NonExpansive (NatOpRSCtx op β).
+  #[local] Instance NatOpRSCtx_ne op (β : IT) `{!SubOfe natO A} : NonExpansive (NatOpRSCtx op β).
   Proof.
     intro n. unfold NatOpRSCtx.
     repeat intro. by apply (NATOP _ β).
     (* XXX why doesn't f_equiv work here? *)
   Qed.
-  #[export] Instance NatOpRSCtx_hom op (β : IT) : IT_hom (NatOpRSCtx op β).
+  #[export] Instance NatOpRSCtx_hom op (β : IT) `{!SubOfe natO A} : IT_hom (NatOpRSCtx op β).
   Proof.
     unfold NatOpRSCtx.
     simple refine (IT_HOM _ _ _ _ _).
@@ -280,9 +405,9 @@ Section lambda.
       repeat f_equiv. intro. reflexivity.
     - intros e. simpl. rewrite NATOP_Err_r//.
   Qed.
-  #[local] Instance IFSCtx_ne (β1 β2 : IT) : NonExpansive (IFSCtx β1 β2).
+  #[local] Instance IFSCtx_ne (β1 β2 : IT) `{!SubOfe natO A} : NonExpansive (IFSCtx β1 β2).
   Proof. unfold IFSCtx. solve_proper. Qed.
-  #[export] Instance IFSCtx_hom (β1 β2 : IT) : IT_hom (IFSCtx β1 β2).
+  #[export] Instance IFSCtx_hom (β1 β2 : IT) `{!SubOfe natO A} : IT_hom (IFSCtx β1 β2).
   Proof.
     unfold IFSCtx.
     simple refine (IT_HOM _ _ _ _ _).
